lib/exportp4.ml
@@ -52,14 +52,11 @@ let print_nat p n =
 let print_bigint p n =
   fprintf p "%s" (Bignum.to_string_accurate (Bignum.of_bigint n))
 
-let print_bignat p n =
-  fprintf p "%s%%N" (Bignum.to_string_accurate (Bignum.of_bigint n))
-
 let p4int p (n : P4int.t) =
   fprintf p "{| @[<hov 0>itags := %a;@ value := %a;@ width_signed := %a |}@]" 
       print_info n.tags 
       print_bigint n.value
-      (print_option (print_pair print_bignat print_bool)) n.width_signed
+      (print_option (print_pair print_nat print_bool)) n.width_signed
 
 let print_direction p (dir: direction) =
   let s = 
@@ -101,17 +98,17 @@ let rec print_type p (typ : coq_P4Type) =
       fprintf p "@[<hov 0>TypInteger@]"
   | TypInt width ->
       fprintf p "(@[<hov 0>TypInt@ %a)@]"
-          print_bigint width
+          print_nat width
   | TypBit width ->
       fprintf p "(@[<hov 0>TypBit@ %a)@]"
-          print_bigint width
+          print_nat width
   | TypVarBit width ->
       fprintf p "(@[<hov 0>TypVarBit@ %a)@]"
-          print_bigint width
+          print_nat width
   | TypArray (typ, size) ->
       fprintf p "(@[<hov 4>TypArray@ %a@ %a)@]"
           print_type typ
-          print_bigint size
+          print_nat size
   | TypTuple typs ->
       fprintf p "(@[<hov 0>TypTuple@ %a)@]"
           (print_list print_type) typs
@@ -208,7 +205,7 @@ and print_param p (param: coq_P4Parameter) =
           print_bool opt
           print_direction direction
           print_type typ
-          (print_option print_bigint) default_arg_id
+          (print_option print_nat) default_arg_id
           p4string variable
 
 let print_types =
@@ -372,10 +369,19 @@ and print_pre_expr p (pre_expr : coq_ExpressionPreT) =
           (print_list print_expr) args
   | ExpDontCare ->
     fprintf p "@[<hov 0>ExpDontCare@]"
+  | ExpMask (expr, mask) ->
+      fprintf p "(@[<hov 4>ExpMask@ %a@ %a)@]"
+          print_expr expr
+          print_expr mask
+  | ExpRange (lo, hi) -> 
+      fprintf p "(@[<hov 4>ExpRange@ %a@ %a)@]"
+          print_expr lo
+          print_expr hi
 and print_keyvalue p kv =
   match kv with
-  | (key, value) ->
-      fprintf p "(@[<hov 4>(%a@, %a)@]"
+  | MkKeyValue (info, key, value) ->
+      fprintf p "(@[<hov 4>MkKeyValue@ %a@ %a@ %a)@]"
+          print_info info
           p4string key
           print_expr value
 
@@ -386,17 +392,8 @@ let print_pre_match p (m: coq_MatchPreT) =
   match m with
   | MatchDontCare -> 
       fprintf p "@[<hov 0>MatchDontCare@]"
-  | MatchMask (expr, mask) ->
-     fprintf p "(@[<hov 0>MatchMask@ %a %a)@]"
-       print_expr expr
-       print_expr mask
-  | MatchRange (lo, hi) ->
-     fprintf p "(@[<hov 0>MatchRange@ %a %a)@]"
-       print_expr lo
-       print_expr hi
-  | MatchCast (typ, expr) ->
-     fprintf p "(@[<hov 0>MatchCast@ %a %a)@]"
-       print_type typ
+  | MatchExpression expr -> 
+      fprintf p "(@[<hov 0>MatchExpression@ %a)@]"
           print_expr expr
 
 let print_match p (m: coq_Match) =
@@ -459,6 +456,103 @@ let print_table_property p (property: coq_TableProperty) =
           p4string s
           print_expr expr
 
+let rec print_value_base p (value : coq_ValueBase)=
+  match value with
+  | ValBaseNull ->
+      fprintf p "@[<hov 0>ValBaseNull@]"
+  | ValBaseBool b ->
+      fprintf p "(@[<hov 0>ValBaseBool@ %a)@]"
+          print_bool b
+  | ValBaseInteger n ->
+      fprintf p "(@[<hov 0>ValBaseInteger@ %a)@]" 
+          print_bigint n
+  | ValBaseBit (width, value) ->
+      fprintf p "(@[<hov 4>ValBaseBit@ %a@ %a)@]" 
+          print_nat width
+          print_bigint value
+  | ValBaseInt (width, value) ->
+      fprintf p "(@[<hov 4>ValBaseInt@ %a@ %a)@]" 
+          print_nat width
+          print_bigint value
+  | ValBaseVarbit (max, width, value) ->
+      fprintf p "(@[<hov 4>ValBaseVarbit@ %a@ %a@ %a)@]" 
+          print_nat max
+          print_nat width
+          print_bigint value
+  | ValBaseString s ->
+      fprintf p "(@[<hov 0>ValBaseString@ %a)@]" 
+          p4string s
+  | ValBaseTuple values ->
+      fprintf p "(@[<hov 0>ValBaseTuple@ %a)@]"
+          (print_list print_value_base) values
+  | ValBaseRecord fields ->
+      fprintf p "(@[<hov 0>ValBaseRecord@ %a)@]"
+          (print_list (print_pair p4string print_value_base)) fields
+  | ValBaseSet value_set ->
+      fprintf p "(@[<hov 0>ValBaseSet@ %a)@]"
+          print_value_set value_set
+  | ValBaseError s ->
+      fprintf p "(@[<hov 0>ValBaseError@ %a)@]"
+          p4string s
+  | ValBaseMatchKind s ->
+      fprintf p "(@[<hov 0>ValBaseMatchKind@ %a)@]"
+          p4string s
+  | ValBaseStruct fields ->
+      fprintf p "(@[<hov 0>ValBaseStruct@ %a)@]"
+          (print_list (print_pair p4string print_value_base)) fields
+  | ValBaseHeader (fields, is_valid )->
+      fprintf p "(@[<hov 4>ValBaseHeader@ %a@ %a)@]"
+          (print_list (print_pair p4string print_value_base)) fields
+          print_bool is_valid
+  | ValBaseUnion fields ->
+      fprintf p "(@[<hov 0>ValBaseUnion@ %a)@]"
+          (print_list (print_pair p4string print_value_base)) fields
+  | ValBaseStack (headers, size, next) ->
+      fprintf p "(@[<hov 4>ValBaseStack@ %a@ %a@ %a)@]"
+          (print_list print_value_base) headers
+          print_nat size
+          print_nat next
+  | ValBaseEnumField (typ_name, enum_name) ->
+      fprintf p "(@[<hov 4>ValBaseEnumField@ %a@ %a)@]"
+          p4string typ_name
+          p4string enum_name
+  | ValBaseSenumField (typ_name, enum_name, value) ->
+      fprintf p "(@[<hov 4>ValBaseSenumField@ %a@ %a@ %a)@]"
+          p4string typ_name
+          p4string enum_name
+          print_value_base value
+  | ValBaseSenum fields -> 
+      fprintf p "(@[<hov 0>ValBaseSenum@ %a)@]"
+          (print_list (print_pair p4string print_value_base)) fields
+and print_value_set p (val_set: coq_ValueSet) =
+  match val_set with
+  | ValSetSingleton value ->
+      fprintf p "(@[<hov 4>ValSetSingleton@ %a)@]"
+          print_value_base value
+  | ValSetUniversal ->
+      fprintf p "@[<hov 4>ValSetUniversal@]"
+  | ValSetMask (value, mask) ->
+      fprintf p "(@[<hov 4>ValSetMask@ %a@ %a)@]" 
+          print_value_base value
+          print_value_base mask
+  | ValSetRange (lo, hi) ->
+      fprintf p "(@[<hov 4>ValSetRange@ %a@ %a)@]" 
+          print_value_base lo
+          print_value_base hi
+  | ValSetProd val_sets ->
+      fprintf p "(@[<hov 0>ValSetProd@ %a)@]"
+          (print_list print_value_set) val_sets
+  | ValSetLpm (width, num_bits, value) ->
+      fprintf p "(@[<hov 4>ValSetLpm@ %a@ %a@ %a)@]" 
+          print_value_base width
+          print_nat num_bits
+          print_value_base value
+  | ValSetValueSet (size, members, val_sets) ->
+      fprintf p "(@[<hov 4>ValSetValueSet@ %a@ %a@ %a)@]" 
+          print_value_base size
+          (print_list print_matches) members
+          (print_list print_value_set) val_sets
+
 let print_stmt_switch_label p (label: coq_StatementSwitchLabel) =
   match label with
   | StatSwLabDefault info -> 
@@ -518,7 +612,7 @@ and print_pre_stmt p (pre_stmt: coq_StatementPreT) =
       fprintf p "(@[<hov 4>StatConstant@ %a@ %a@ %a@ %a)@]"
           print_type typ
           p4string s
-          print_expr value
+          print_value_base value
           print_locator loc
   | StatVariable (typ, s, init, loc) ->
       fprintf p "(@[<hov 4>StatVariable@ %a@ %a@ %a@ %a)@]"
@@ -638,7 +732,7 @@ let rec print_decl (decl_name : string option) p (decl : coq_Declaration) =
           print_info info
           print_type typ
           p4string name
-          print_expr value
+          print_value_base value
   | DeclInstantiation (info, typ, args, name, init) ->
       let (f_str, decl_name) = 
         (gen_format_string decl_name "DeclInstantiation@ %a@ %a@ %a@ %a@ %a")
@@ -715,7 +809,7 @@ let rec print_decl (decl_name : string option) p (decl : coq_Declaration) =
           decl_name
           print_info info
           print_type typ
-          print_bigint size
+          print_expr size
           p4string name
   | DeclAction (info, name, data_params, ctrl_params, body) ->
       let (f_str, decl_name) = 
@@ -741,7 +835,7 @@ let rec print_decl (decl_name : string option) p (decl : coq_Declaration) =
           print_table_actions actions
           (print_option print_table_entries) entries
           (print_option print_table_action_ref) default_action
-          (print_option print_bigint) size
+          (print_option p4int) size
           (print_list print_table_property) custom_properties
   | DeclHeader (info, name, fields) ->
       let (f_str, decl_name) = 
@@ -948,13 +1042,151 @@ let print_top_decl p (existing: string list) (decl : coq_Declaration): string =
 let print_value_loc =
   p4string
 
+let print_value_table p (value_table: coq_ValueTable) =
+  match value_table with
+  | MkValTable (name, keys, actions, default_action, const_entries) ->
+      fprintf p "(@[<hov 4>MkValTable@ %a@ %a@ %a@ %a@ %a)@]"
+          p4string name
+          print_table_keys keys
+          print_table_actions actions
+          print_table_action_ref default_action
+          print_table_entries const_entries
+
 let print_env_env print_binding =
   print_list (print_list (print_pair p4string print_binding))
+
+let print_env_eval_env p (env: coq_Env_EvalEnv) =
+  match env with
+  | MkEnv_EvalEnv (vs, typ, namespaces) ->
+      fprintf p "(@[<hov 4>MkEnv_EvalEnv@ %a@ %a@ %a)@]"
+          (print_env_env p4string) vs
+          (print_env_env print_type) typ
+          p4string namespaces
+  
+let rec print_value_pre_lvalue p (lvalue : coq_ValuePreLvalue) = 
+  match lvalue with
+  | ValLeftName (name, loc) ->
+      fprintf p "(@[<hov 0>ValLeftName@ %a@ %a)@]"
+          print_name name
+          print_locator loc
+  | ValLeftMember (expr, name) ->
+      fprintf p "(@[<hov 4>ValLeftMember@ %a@ %a)@]"
+          print_lvalue expr
+          p4string name
+  | ValLeftBitAccess (expr, msb, lsb) ->
+      fprintf p "(@[<hov 4>ValLeftBitAccess@ %a@ %a@ %a)@]"
+          print_lvalue expr
+          print_nat msb
+          print_nat lsb
+  | ValLeftArrayAccess (expr, idx) ->
+      fprintf p "(@[<hov 4>ValLeftArrayAccess@ %a@ %a)@]"
+          print_lvalue expr
+          print_nat idx
+and print_lvalue p (lvalue: coq_ValueLvalue) =
+  match lvalue with
+  | MkValueLvalue  (lvalue, typ) ->
+      fprintf p "(@[<hov 4>MkValueLvalue@ %a@ %a)@]"
+          print_value_pre_lvalue lvalue
+          print_type typ
+  
+let print_value_fun_imp p (val_fun_impl: coq_ValueFunctionImplementation) =
+  match val_fun_impl with
+  | ValFuncImplUser (scope, body) ->
+      fprintf p "(@[<hov 4>ValFuncImplUser@ %a@ %a)@]"
+          print_env_eval_env scope
+          print_block body
+  | ValFuncImplExtern (name, caller) ->
+      fprintf p "(@[<hov 4>ValFuncImplExtern@ %a@ %a)@]"
+          p4string name
+          (print_option (print_pair print_value_loc p4string)) caller
+  | ValFuncImplBuiltin (name, caller) ->
+      fprintf p "(@[<hov 4>ValFuncImplExtern@ %a@ %a)@]"
+          p4string name
+          print_lvalue caller
+
+let print_value_object p (value: coq_ValueObject) =
+  match value with
+  | ValObjParser (scope, constructor_params, params, locals, states) ->
+      fprintf p "(@[<hov 4>ValObjParser@ %a@ %a@ %a@ %a@ %a)@]"
+          print_env_eval_env scope
+          print_params constructor_params
+          print_params params
+          print_decls locals
+          print_parser_states states
+  | ValObjTable (value_table) ->
+      fprintf p "(@[<hov 0>ValObjTable@ %a)@]"
+          print_value_table value_table
+  | ValObjControl (scope, constructor_params, params, locals, apply) ->
+      fprintf p "(@[<hov 4>ValObjControl@ %a@ %a@ %a@ %a@ %a)@]"
+          print_env_eval_env scope
+          print_params constructor_params
+          print_params params
+          print_decls locals
+          print_block apply
+  | ValObjPackage args ->
+      fprintf p "(@[<hov 0>ValObjPackage@ %a)@]"
+          (print_list (print_pair p4string print_value_loc)) args
+  | ValObjRuntime (loc, obj_name) ->
+      fprintf p "(@[<hov 4>ValObjRuntime@ %a@ %a)@]"
+          print_value_loc loc
+          p4string obj_name
+  | ValObjFun (params, imp) ->
+      fprintf p "(@[<hov 4>ValObjFun@ %a@ %a)@]"
+          print_params params
+          print_value_fun_imp  imp
+  | ValObjAction (scope, params, body) ->
+      fprintf p "(@[<hov 4>ValObjAction@ %a@ %a@ %a)@]"
+          print_env_eval_env scope
+          print_params params
+          print_block body
+  | ValObjPacket bits ->
+      fprintf p "(@[<hov 0>ValObjPacket@ %a)@]"
+          (print_list print_bool) bits
+
+let print_value_constructor p (value: coq_ValueConstructor) =
+  match value with
+  | ValConsParser (scope, constructor_params, params, locals, states) ->
+      fprintf p "(@[<hov 4>ValConsParser@ %a@ %a@ %a@ %a@ %a)@]"
+          print_env_eval_env scope
+          print_params constructor_params
+          print_params params
+          print_decls locals
+          print_parser_states states
+  | ValConsTable (value_table) ->
+      fprintf p "(@[<hov 0>ValConsTable@ %a)@]"
+          print_value_table value_table
+  | ValConsControl (scope, constructor_params, params, locals, apply) ->
+      fprintf p "(@[<hov 4>ValConsControl@ %a@ %a@ %a@ %a@ %a)@]"
+          print_env_eval_env scope
+          print_params constructor_params
+          print_params params
+          print_decls locals
+          print_block apply
+  | ValConsPackage (params, args) ->
+      fprintf p "(@[<hov 4>ValConsPackage@ %a@ %a)@]"
+          print_params params
+          (print_list (print_pair p4string print_value_loc)) args
+  | ValConsExternObj fields ->
+      fprintf p "(@[<hov 0>ValConsExternObj@ %a)@]"
+          (print_list (print_pair p4string (print_params))) fields
+
+let print_value p (value: coq_Value) =
+  match value with
+  | ValBase value ->
+      fprintf p "(@[<hov 0>ValBase@ %a)@]"
+          print_value_base value
+  | ValObj value ->
+      fprintf p "(@[<hov 0>ValBase@ %a)@]"
+          print_value_object value
+  | ValCons value ->
+      fprintf p "(@[<hov 0>ValCons@ %a)@]"
+          print_value_constructor value
 
 let print_header p =
   fprintf p "Require Import Poulet4.P4defs.@ ";
   fprintf p "Open Scope string_scope.@ @ ";
   fprintf p "Import ListNotations.@ @ "
+
 
 let print_program p (program : Prog.program) =
   fprintf p "@[<v 0>";
