lib/lexer.mll
@@ -94,9 +94,9 @@ let parse_width_int s n info =
       "s" ->
       if (int_of_string width < 2)
       then raise (Error "signed integers must have width at least 2")
-      else Some (Bigint.of_string width, true)
+      else Some (int_of_string width, true)
     | "w" ->
-      Some (Bigint.of_string width, false)
+      Some (int_of_string width, false)
     | _ -> 
       raise (Error "Illegal integer constant")
   in
