lib/ops.mli
@@ -1,6 +1,6 @@
 open Typed
 open Prog
     
-val interp_binary_op: coq_OpBin -> coq_Value -> coq_Value -> coq_Value
-val interp_unary_op: coq_OpUni -> coq_Value -> coq_Value
-val interp_cast: type_lookup:(P4name.t -> coq_P4Type) -> coq_P4Type -> coq_Value -> coq_Value
+val interp_binary_op: coq_OpBin -> coq_ValueBase -> coq_ValueBase -> coq_ValueBase
+val interp_unary_op: coq_OpUni -> coq_ValueBase -> coq_ValueBase
+val interp_cast: type_lookup:(P4name.t -> coq_P4Type) -> coq_P4Type -> coq_ValueBase -> coq_ValueBase
