lib/typed.ml
@@ -23,7 +23,6 @@ type coq_ExprContext = [%import:Poulet4.Typed.coq_ExprContext]
 type 'a pre_P4Type =
   [%import:'a Poulet4.Typed.coq_P4Type
     [@with name := P4name.pre_t;
-           Bigint.t := Util.bigint;
            Poulet4.P4String.t := P4string.pre_t;
            coq_ControlType := pre_ControlType;
            coq_P4Parameter := pre_P4Parameter;
@@ -45,7 +44,6 @@ and 'a pre_ControlType =
 and pre_P4Parameter =
   [%import:'a Poulet4.Typed.coq_P4Parameter
     [@with Poulet4.P4String.t := P4string.pre_t;
-           Bigint.t := Util.bigint;
            coq_P4Type := pre_P4Type]]
   [@@deriving sexp,show,yojson]
 type coq_P4Type = Info.t pre_P4Type
