deps/poulet4/lib/Environment/Environment.v
@@ -2,7 +2,6 @@ Require Import Coq.Lists.List.
 Require Import Coq.FSets.FMapList.
 Require Import Coq.Structures.OrderedTypeEx.
 Require Import Coq.ZArith.BinIntDef.
-Require Import Coq.NArith.BinNat.
 Require Import Coq.Strings.String.
 
 Require Import Poulet4.Monads.Monad.
@@ -12,7 +11,7 @@ Require Import Poulet4.Monads.Transformers.
 
 Require Import Poulet4.Bitwise.
 Require Import Poulet4.Typed.
-Require Import Poulet4.Value.
+Require Import Poulet4.Syntax.
 Require Import Poulet4.P4String.
 Require Poulet4.StringConstants.
 
@@ -38,12 +37,11 @@ Section Environment.
 
   Context (tags_t: Type).
   Context (tags_dummy: tags_t).
-  Context (bit: Type).
 
   Definition loc := nat.
   Definition scope := MStr.t loc.
   Definition stack := list scope.
-  Definition heap := MNat.t (@Value tags_t bit).
+  Definition heap := MNat.t (@Value tags_t).
 
   Record environment := MkEnvironment {
     env_fresh: loc;
@@ -114,21 +112,21 @@ Section Environment.
         |}
       end.
 
-  Definition heap_lookup (l: loc) : env_monad (@Value tags_t bit) :=
+  Definition heap_lookup (l: loc) : env_monad (@Value tags_t) :=
     fun env =>
       match MNat.find l (env_heap env) with
       | None => state_fail (AssertError "Unable to look up location on heap.") env
       | Some val => mret val env
       end.
 
-  Definition heap_update (l: loc) (v: @Value tags_t bit) : env_monad unit :=
+  Definition heap_update (l: loc) (v: @Value tags_t) : env_monad unit :=
     fun env => mret tt {|
       env_fresh := env_fresh env;
       env_stack := env_stack env;
       env_heap := MNat.add l v (env_heap env);
     |}.
 
-  Definition heap_insert (v: @Value tags_t bit) : env_monad loc :=
+  Definition heap_insert (v: @Value tags_t) : env_monad loc :=
     fun env =>
       let l := env_fresh env in
       mret l {|
@@ -137,7 +135,7 @@ Section Environment.
         env_heap := MNat.add l v (env_heap env);
       |}.
 
-  Definition env_insert (name: string) (v: @Value tags_t bit) : env_monad unit :=
+  Definition env_insert (name: string) (v: @Value tags_t) : env_monad unit :=
     let* l := heap_insert v in
     stack_insert name l.
 
@@ -148,41 +146,36 @@ Section Environment.
     | _ :: scopes' => top_scope scopes'
     end.
 
-  Definition lookup_value (v: @ValueBase tags_t bit) (field: P4String.t tags_t) : @option_monad (@ValueBase tags_t bit) :=
+  Definition lookup_value (v: @ValueBase tags_t) (field: P4String.t tags_t) : @option_monad (@ValueBase tags_t) :=
     match v with
     | ValBaseRecord fields
     | ValBaseStruct fields
     | ValBaseUnion fields
-    | ValBaseHeader fields _ => AList.get fields field
-    (*| ValBaseSenum fields => AList.get fields field*)
+    | ValBaseHeader fields _
+    | ValBaseSenum fields => AList.get fields field
     | ValBaseStack hdrs len next =>
-      if eq_const field StringConstants.last then List.nth_error hdrs (N.to_nat (len - 1)) else
-      if eq_const field StringConstants.next then List.nth_error hdrs (N.to_nat next) else
+      if eq_const field StringConstants.last then List.nth_error hdrs (len - 1) else
+      if eq_const field StringConstants.next then List.nth_error hdrs next else
       None
     | _ => None
     end.
 
-  Definition bit_slice (v: @ValueBase tags_t bit) (msb lsb: N) : @option_monad (@ValueBase tags_t bit) :=
+  Definition bit_slice (v: @ValueBase tags_t) (msb: nat) (lsb: nat): @option_monad (@ValueBase tags_t) :=
     match v with
-    | ValBaseBit bits
-    | ValBaseInt bits =>
-      let width := N.of_nat (List.length bits) in
-      if (lsb <=? msb) && (msb <=? width)
-      then
-        let* sliced := slice (N.to_nat width) bits (N.to_nat lsb) (N.to_nat msb) in
-        Some (ValBaseBit sliced)
-      else None
-    | ValBaseVarbit width bits =>
-      if (lsb <=? msb) && (msb <=? width)
+    | ValBaseBit width val
+    | ValBaseInt width val
+    | ValBaseVarbit _ width val =>
+      if Nat.leb lsb msb && Nat.leb msb width
       then
         let w_out := msb - lsb in
-        let* sliced := slice (N.to_nat width) bits (N.to_nat lsb) (N.to_nat msb) in
-        Some (ValBaseBit sliced)
+        let bits := of_nat (Z.to_nat val) width in
+        let* sliced := slice width bits lsb msb in
+        Some (ValBaseBit w_out (Z.of_nat (to_nat sliced)))
       else None
     | _ => None
     end.
 
-  Definition array_index (v: @ValueBase tags_t bit) (idx: nat): @option_monad (@ValueBase tags_t bit) :=
+  Definition array_index (v: @ValueBase tags_t) (idx: nat): @option_monad (@ValueBase tags_t) :=
     match v with
     | ValBaseStack hdrs _ _ => nth_error hdrs idx
     | _ => None
@@ -199,40 +192,40 @@ Section Environment.
       state_fail (SupportError "Qualified name lookup is not implemented.")
     end.
 
-  Definition env_name_lookup (name: Typed.name) : env_monad (@Value tags_t bit) :=
+  Definition env_name_lookup (name: Typed.name) : env_monad (@Value tags_t) :=
     get_name_loc name >>= heap_lookup.
 
-  Definition env_str_lookup (name: P4String.t tags_t) : env_monad (@Value tags_t bit) :=
+  Definition env_str_lookup (name: P4String.t tags_t) : env_monad (@Value tags_t) :=
     env_name_lookup (BareName name).
 
-  Definition env_dig (val: @Value tags_t bit) (lval: @ValuePreLvalue tags_t) : option_monad :=
+  Definition env_dig (val: @Value tags_t) (lval: @ValuePreLvalue tags_t) : option_monad :=
     match lval with
     | ValLeftName _ _ => Some val
     | ValLeftMember _ member =>
       match val with
-      | ValBase _ v =>
+      | ValBase v =>
         let* v' := lookup_value v member in
-        Some (ValBase _ v')
+        Some (ValBase v')
       | _ => None
       end
     | ValLeftBitAccess _ msb lsb =>
       match val with
-      | ValBase _ v =>
+      | ValBase v =>
         let* v' := bit_slice v msb lsb in
-        Some (ValBase _ v')
+        Some (ValBase v')
       | _ => None
       end
     | ValLeftArrayAccess _ idx =>
       match val with
-      | ValBase _ v =>
-        let* v' := array_index v (N.to_nat idx) in
-        Some (ValBase _ v')
+      | ValBase v =>
+        let* v' := array_index v idx in
+        Some (ValBase v')
       | _ => None
       end
     end
   .
 
-  Fixpoint env_lookup (lvalue: @ValueLvalue tags_t) : env_monad (@Value tags_t bit) :=
+  Fixpoint env_lookup (lvalue: @ValueLvalue tags_t) : env_monad (@Value tags_t) :=
     let 'MkValueLvalue lv _ := lvalue in
     let* val_inner := match lv with
     | ValLeftName name _ => env_name_lookup name
@@ -244,14 +237,12 @@ Section Environment.
     lift_opt (AssertError "Could not dig into value.") (env_dig val_inner lv)
   .
 
-  Definition update_slice (lhs: @ValueBase tags_t bit) (msb: nat) (lsb: nat) (rhs: @ValueBase tags_t bit) : env_monad (@ValueBase tags_t bit) :=
+  Definition update_slice (lhs: @ValueBase tags_t) (msb: nat) (lsb: nat) (rhs: @ValueBase tags_t) : env_monad (@ValueBase tags_t) :=
     match (lhs, rhs) with
-    | (ValBaseBit vl, ValBaseBit vr) =>
-      let wl := List.length vl in
-      let wr := List.length vr in
-      let* bit_result := lift_opt (AssertError "Could not splice bits.")
-                                  (splice wl vl lsb msb wr vr) in
-      state_return (ValBaseBit bit_result)
+    | (ValBaseBit wl vl, ValBaseBit wr vr) =>
+      let (bitl, bitr) := (of_nat (Z.to_nat vl) wl, of_nat (Z.to_nat vr) wr) in
+      let* bit_result := lift_opt (AssertError "Could not splice bits.") (splice wl bitl lsb msb wr bitr) in
+      state_return (ValBaseBit wl (Z.of_nat (to_nat bit_result)))
     | _ => state_fail (TypeError "Bit slice update requires bit values on both sides.")
     end.
 
@@ -261,16 +252,16 @@ Section Environment.
   Definition split_list {A} (idx: nat) (xs: list A) : (list A * list A) :=
     (firstn idx xs, skipn (List.length xs - idx) xs).
 
-  Definition update_array (lhs: @ValueBase tags_t bit) (idx: nat) (rhs: @ValueBase tags_t bit) : env_monad (@ValueBase tags_t bit) :=
+  Definition update_array (lhs: @ValueBase tags_t) (idx: nat) (rhs: @ValueBase tags_t) : env_monad (@ValueBase tags_t) :=
     match lhs with
     | ValBaseStack hdrs len nxt =>
-      if N.leb len (N.of_nat idx) then state_fail (AssertError "Out of bounds header stack write.") else
+      if Nat.leb len idx then state_fail (AssertError "Out of bounds header stack write.") else
       let (pref, suff) := split_list idx hdrs in
       state_return (ValBaseStack (pref ++ rhs :: suff) len nxt)
     | _ => state_fail (TypeError "Attempt to update something that is not a header stack.")
     end.
 
-  Definition update_member (lhs: @ValueBase tags_t bit) (member: @P4String.t tags_t) (rhs: @ValueBase tags_t bit) : env_monad (@ValueBase tags_t bit) :=
+  Definition update_member (lhs: @ValueBase tags_t) (member: @P4String.t tags_t) (rhs: @ValueBase tags_t) : env_monad (@ValueBase tags_t) :=
     match lhs with
     (* TODO: there must be a cleaner way... *)
     | ValBaseRecord fields =>
@@ -289,18 +280,18 @@ Section Environment.
       let* fields' := lift_opt (AssertError "Unable to update member of union")
                                (AList.set fields member rhs) in
       state_return (ValBaseRecord fields')
-    (*| ValBaseSenum fields =>
+    | ValBaseSenum fields =>
       let* fields' := lift_opt (AssertError "Unable to update member of enum.")
                                (AList.set fields member rhs) in
-      state_return (ValBaseSenum fields')*)
+      state_return (ValBaseSenum fields')
     | ValBaseStack hdrs len next =>
-      if eq_const member StringConstants.last then update_array lhs (N.to_nat len) rhs else
-      if eq_const member StringConstants.next then update_array lhs (N.to_nat next) rhs else
+      if eq_const member StringConstants.last then update_array lhs len rhs else
+      if eq_const member StringConstants.next then update_array lhs next rhs else
       state_fail (AssertError "Can only update next and last members of header stack.")
     | _ => state_fail (AssertError "Unsupported value in member update.")
     end.
 
-  Fixpoint env_update (lvalue: @ValueLvalue tags_t) (value: @Value tags_t bit) : env_monad unit :=
+  Fixpoint env_update (lvalue: @ValueLvalue tags_t) (value: @Value tags_t) : env_monad unit :=
     let 'MkValueLvalue lv _ := lvalue in
     match lv with
     | ValLeftName nm _ =>
@@ -311,40 +302,40 @@ Section Environment.
     | ValLeftMember inner member =>
       let* lv' := env_lookup inner in
       match (lv', value) with
-      | (ValBase _ lv'', ValBase _ value') =>
+      | (ValBase lv'', ValBase value') =>
         let* value'' := update_member lv'' member value' in
-        env_update inner (ValBase _ value'')
+        env_update inner (ValBase value'')
       | _ => state_fail (TypeError "Member expression did not evaluate to base values.")
       end
     | ValLeftBitAccess inner msb lsb =>
       let* lv' := env_lookup inner in
       match (lv', value) with
-      | (ValBase _ lv'', ValBase _ value') =>
-        let* value'' := update_slice lv'' (N.to_nat msb) (N.to_nat lsb) value' in
-        env_update inner (ValBase _ value'')
+      | (ValBase lv'', ValBase value') =>
+        let* value'' := update_slice lv'' msb lsb value' in
+        env_update inner (ValBase value'')
       | _ => state_fail (TypeError "Bit access expression did not evaluate to base values.")
       end
     | ValLeftArrayAccess inner idx =>
       let* lv' := env_lookup inner in
       match (lv', value) with
-      | (ValBase _ lv'', ValBase _ value') =>
-        let* value'' := update_array lv'' (N.to_nat idx) value' in
-        env_update inner (ValBase _ value'')
+      | (ValBase lv'', ValBase value') =>
+        let* value'' := update_array lv'' idx value' in
+        env_update inner (ValBase value'')
       | _ => state_fail (TypeError "Array access expression did not evaluate to base values.")
       end
     end.
 
-  Definition toss_value (original: env_monad (@Value tags_t bit)) : env_monad unit :=
+  Definition toss_value (original: env_monad (@Value tags_t)) : env_monad unit :=
     fun env =>
       match original env with
       | (inl result, env') => mret tt env'
       | (inr exc, env') => state_fail exc env'
       end.
 
-  Definition dummy_value (original: env_monad unit) : env_monad (@Value tags_t bit) :=
+  Definition dummy_value (original: env_monad unit) : env_monad (@Value tags_t) :=
     fun env =>
       match original env with
-      | (inl tt, env') => mret (ValBase _ ValBaseNull) env'
+      | (inl tt, env') => mret (ValBase ValBaseNull) env'
       | (inr exc, env') => state_fail exc env'
       end.
 End Environment.
