deps/poulet4/lib/P4cub/BigStep/ExprUtil.v
@@ -1,6 +1,6 @@
 Set Warnings "-custom-entry-overridden".
 Require Import Poulet4.P4Arith Poulet4.P4cub.BigStep.Value.Value
-        Coq.Bool.Bool Coq.ZArith.BinInt Coq.NArith.BinNat
+        Coq.Bool.Bool Coq.ZArith.BinInt
         Coq.Arith.Compare_dec Coq.micromega.Lia
         Poulet4.P4cub.Syntax.Auxilary.
 Require Poulet4.P4cub.Static.Util.
@@ -11,7 +11,7 @@ Definition eval_slice (hi lo : positive) (v : Val.v) : option Val.v :=
   match v with
   | ~{ _ VW z }~
   | ~{ _ VS z }~
-    => let w' := (Npos hi - Npos lo + 1)%N in
+    => let w' := (hi - lo + 1)%positive in
       Some $ Val.VBit w' $
            BitArith.mod_bound w' $
            BitArith.bitstring_slice z hi lo
@@ -32,7 +32,8 @@ Definition eval_uop (op : Expr.uop) (v : Val.v) : option Val.v :=
     => Some ~{ HDR { vs } VALID:=true }~
   | _{ setInValid }_, ~{ HDR { vs } VALID:=_ }~
     => Some ~{ HDR { vs } VALID:=false }~
-  | _{ Size }_, ~{ STACK _:_ NEXT:=_ }~ => Some $ Val.VBit 32%N $ 0%Z
+  | _{ Size }_, ~{ STACK hs:_ NEXT:=_ }~ =>
+    Some $ Val.VBit 32%positive $ Z.of_nat $ length hs
   | _{ Next }_, ~{ STACK hs:_ NEXT:=ni }~
     => bvs <<| nth_error hs $ Z.to_nat ni ;;
       match bvs with
@@ -98,17 +99,11 @@ Definition eval_bop (op : Expr.bop) (v1 v2 : Val.v) : option Val.v :=
   | +{ == }+, _, _ => Some $ Val.VBool $ eqbv v1 v2
   | +{ != }+, _, _ => Some $ Val.VBool $ negb $ eqbv v1 v2
   | +{ ++ }+, ~{ w1 VW n1 }~, ~{ w2 VW n2 }~
-    => Some $ Val.VBit (w1 + w2)%N $ BitArith.concat w1 w2 n1 n2
   | +{ ++ }+, ~{ w1 VW n1 }~, ~{ w2 VS n2 }~
-    => Some $ Val.VBit (w1 + Npos w2)%N $ BitArith.concat w1 (Npos w2) n1 n2
+    => Some $ Val.VBit (w1 + w2)%positive $ BitArith.concat w1 w2 n1 n2
   | +{ ++ }+, ~{ w1 VS n1 }~, ~{ w2 VS n2 }~
-    => Some $ Val.VInt (w1 + w2)%positive $ IntArith.concat (Npos w1) (Npos w2) n1 n2
   | +{ ++ }+, ~{ w1 VS n1 }~, ~{ w2 VW n2 }~
-    =>
-    match w2 with
-    | Npos w2 => Some $ Val.VInt (w1 + w2)%positive $ IntArith.concat (Npos w1) (Npos w2) n1 n2
-    | N0 => Some $ Val.VInt w1 n1
-    end
+    => Some $ Val.VInt (w1 + w2)%positive $ IntArith.concat w1 w2 n1 n2
   | _, _, _ => None
   end.
 (**[]*)
@@ -116,10 +111,10 @@ Definition eval_bop (op : Expr.bop) (v1 v2 : Val.v) : option Val.v :=
 Definition eval_cast
            (target : Expr.t) (v : Val.v) : option Val.v :=
   match target, v with
-  | (Expr.TBit (Npos xH)), ~{ TRUE }~         => Some (Val.VBit 1%N 1%Z)
-  | (Expr.TBit (Npos xH)), ~{ FALSE }~        => Some (Val.VBit 1%N 0%Z)
-  | {{ Bool }}, Val.VBit 1%N 1%Z => Some ~{ TRUE }~
-  | {{ Bool }}, Val.VBit 1%N 0%Z => Some ~{ FALSE }~
+  | {{ bit<xH> }}, ~{ TRUE }~         => Some (Val.VBit 1%positive 1%N)
+  | {{ bit<xH> }}, ~{ FALSE }~        => Some (Val.VBit 1%positive 0%N)
+  | {{ Bool }}, Val.VBit 1%positive 1%N => Some ~{ TRUE }~
+  | {{ Bool }}, Val.VBit 1%positive 0%N => Some ~{ FALSE }~
   | {{ bit<w> }}, ~{ _ VS z }~ => let n := BitArith.mod_bound w z in
                                  Some ~{ w VW n }~
   | {{ int<w> }}, ~{ _ VW n }~ => let z := IntArith.mod_bound w n in
@@ -150,14 +145,14 @@ Section Lemmas.
   Section HelpersType.
     Local Hint Constructors type_value : core.
     
-    Lemma eval_member_types : forall x v v' ts τ τ',
+    Lemma eval_member_types : forall  x v v' ts τ τ',
         eval_member x v = Some v' ->
         member_type ts τ ->
         F.get x ts = Some τ' ->
         ∇  ⊢ v ∈ τ ->
         ∇  ⊢ v' ∈ τ'.
     Proof.
-      intros x v v' ts τ τ' Heval Hmem Hget Ht;
+      intros  x v v' ts τ τ' Heval Hmem Hget Ht;
         inv Hmem; inv Ht; unravel in *.
       - eapply F.relfs_get_r in H1 as [? ?]; eauto.
         intuition. rewrite Heval in H0; inv H0; eauto.
@@ -168,23 +163,23 @@ Section Lemmas.
     Local Hint Extern 0 => bit_bounded : core.
     Local Hint Extern 0 => int_bounded : core.
     
-    Lemma eval_slice_types : forall v v' τ hi lo w,
+    Lemma eval_slice_types : forall  v v' τ hi lo w,
         eval_slice hi lo v = Some v' ->
-        (Npos lo <= Npos hi < w)%N ->
+        (lo <= hi < w)%positive ->
         numeric_width w τ ->
-        ∇ ⊢ v ∈ τ ->
-        let w' := (Npos hi - Npos lo + 1)%N in
-        ∇ ⊢ v' ∈ bit<w'>.
+        ∇  ⊢ v ∈ τ ->
+        let w' := (hi - lo + 1)%positive in
+        ∇  ⊢ v' ∈ bit<w'>.
     Proof.
-      intros v v' τ hi lo w Heval Hw Hnum Hv w'; subst w'.
+      intros  v v' τ hi lo w Heval Hw Hnum Hv w'; subst w'.
       inv Hnum; inv Hv; unravel in *; inv Heval; auto 2.
     Qed.
     
-    Lemma eval_bop_type : forall op τ1 τ2 τ v1 v2 v,
+    Lemma eval_bop_type : forall  op τ1 τ2 τ v1 v2 v,
         bop_type op τ1 τ2 τ -> eval_bop op v1 v2 = Some v ->
-        ∇ ⊢ v1 ∈ τ1 -> ∇  ⊢ v2 ∈ τ2 -> ∇ ⊢ v ∈ τ.
+        ∇  ⊢ v1 ∈ τ1 -> ∇  ⊢ v2 ∈ τ2 -> ∇  ⊢ v ∈ τ.
     Proof.
-      intros op τ1 τ2 τ v1 v2 v Hbop Heval Ht1 Ht2; inv Hbop;
+      intros  op τ1 τ2 τ v1 v2 v Hbop Heval Ht1 Ht2; inv Hbop;
         repeat match goal with
                | H: Some _ = Some _ |- _ => inv H; constructor; auto 2
                | H: numeric _ |- _ => inv H
@@ -197,18 +192,18 @@ Section Lemmas.
     
     Local Hint Resolve proper_inside_header_nesting : core.
     
-    Lemma eval_cast_types : forall v v' τ τ',
+    Lemma eval_cast_types : forall  v v' τ τ',
         proper_cast τ τ' -> eval_cast τ' v = Some v' ->
-        ∇ ⊢ v ∈ τ -> ∇ ⊢ v' ∈ τ'.
+        ∇  ⊢ v ∈ τ -> ∇  ⊢ v' ∈ τ'.
     Proof.
-      intros v v' τ τ' Hpc Heval Ht; inv Hpc; inv Ht;
+      intros  v v' τ τ' Hpc Heval Ht; inv Hpc; inv Ht;
         unravel in *; try match goal with
                           | H: Some _ = Some _ |- _ => inv H
                           end; auto 2.
       - destruct b; inv Heval; constructor; cbv; auto 2.
       - destruct n; inv Heval; auto 1; destruct p; inv H0; auto 1.
       - destruct w; inv Heval; auto 2.
-      - destruct w2; [|destruct p]; inv Heval; auto 2.
+      - destruct w2; inv Heval; auto 2.
       - constructor. generalize dependent fs.
         induction vs as [| v vs IHvs]; intros [| [x τ] fs] H;
           inv H; unravel; constructor; unfold F.relf in *;
@@ -235,15 +230,15 @@ Section Lemmas.
     Hint Rewrite @F.relfs_split_map_iff.
     Hint Rewrite @F.map_fst.
     Local Hint Resolve Forall_impl : core.
-    Local Hint Resolve vdefault_types : core.
+    Fail Local Hint Resolve vdefault_types : core.
     Local Hint Resolve Forall_firstn : core.
     Local Hint Resolve Forall_skipn : core.
     
-    Lemma eval_uop_types : forall op τ τ' v v',
+    Lemma eval_uop_types : forall  op τ τ' v v',
         uop_type op τ τ' -> eval_uop op v = Some v' ->
-        ∇ ⊢ v ∈ τ -> ∇ ⊢ v' ∈ τ'.
+        ∇  ⊢ v ∈ τ -> ∇  ⊢ v' ∈ τ'.
     (*Proof.
-      intros op τ τ' v v' Huop Heval Ht;
+      intros  op τ τ' v v' Huop Heval Ht;
         inv Huop; inv Ht; unravel in *; inv Heval; auto 2;
           invert_proper_nesting;
           repeat match goal with
@@ -261,41 +256,41 @@ Section Lemmas.
   End HelpersType.
   
   Section HelpersExist.
-    Lemma eval_slice_exists : forall v τ hi lo w,
-      (Npos lo <= Npos hi < w)%N ->
+    Lemma eval_slice_exists : forall  v τ hi lo w,
+      (lo <= hi < w)%positive ->
       numeric_width w τ ->
-      ∇ ⊢ v ∈ τ ->
+      ∇  ⊢ v ∈ τ ->
       exists v', eval_slice hi lo v = Some v'.
     Proof.
-      intros v τ hi lo w Hw Hnum Hv;
+      intros  v τ hi lo w Hw Hnum Hv;
         inv Hnum; inv Hv; unravel; eauto 2.
     Qed.
     
-    Lemma eval_bop_exists : forall op τ1 τ2 τ v1 v2,
+    Lemma eval_bop_exists : forall  op τ1 τ2 τ v1 v2,
         bop_type op τ1 τ2 τ ->
-        ∇ ⊢ v1 ∈ τ1 -> ∇ ⊢ v2 ∈ τ2 ->
+        ∇  ⊢ v1 ∈ τ1 -> ∇  ⊢ v2 ∈ τ2 ->
         exists v, eval_bop op v1 v2 = Some v.
     Proof.
-      intros op τ1 τ2 τ v1 v2 Hbop Ht1 Ht2; inv Hbop;
+      intros  op τ1 τ2 τ v1 v2 Hbop Ht1 Ht2; inv Hbop;
         repeat inv_numeric; inv Ht1; inv Ht2; unravel; eauto 2;
           try inv_numeric_width.
-    Admitted.
+    Qed.
     
-    Lemma eval_cast_exists : forall τ τ' v,
-        proper_cast τ τ' -> ∇ ⊢ v ∈ τ -> exists v', eval_cast τ' v = Some v'.
+    Lemma eval_cast_exists : forall  τ τ' v,
+        proper_cast τ τ' -> ∇  ⊢ v ∈ τ -> exists v', eval_cast τ' v = Some v'.
     Proof.
-      intros τ τ' v Hpc Ht; inv Hpc; inv Ht; unravel; eauto 2.
+      intros  τ τ' v Hpc Ht; inv Hpc; inv Ht; unravel; eauto 2.
       - destruct b; eauto 2.
       - destruct n; eauto 2; destruct p; eauto 2;
           try (cbv in *; destruct H1; try destruct p; discriminate).
       - destruct w; eauto 2.
       - destruct w2; eauto 2.
-    Admitted.
+    Qed.
     
-    Lemma eval_uop_exist : forall op τ τ' v,
+    Lemma eval_uop_exist : forall  op τ τ' v,
         uop_type op τ τ' -> ∇  ⊢ v ∈ τ -> exists v', eval_uop op v = Some v'.
     (*Proof.
-      intros op τ τ' v Huop Ht; inv Huop; inv Ht;
+      intros  op τ τ' v Huop Ht; inv Huop; inv Ht;
         unravel; repeat inv_numeric; eauto 2;
           try (destruct (lt_dec (Pos.to_nat p) (Pos.to_nat n)) as [? | ?]; eauto 2).
       - assert (Hnith : (Z.to_nat ni < length hs)%nat) by lia;
@@ -304,13 +299,13 @@ Section Lemmas.
     Qed. *)
     Admitted.
       
-    Lemma eval_member_exists : forall x v ts τ τ',
+    Lemma eval_member_exists : forall  x v ts τ τ',
         member_type ts τ ->
         F.get x ts = Some τ' ->
         ∇  ⊢ v ∈ τ ->
         exists v', eval_member x v = Some v'.
     Proof.
-      intros x v ts τ τ' Hmem Hget Ht;
+      intros  x v ts τ τ' Hmem Hget Ht;
         inv Hmem; inv Ht; unravel.
       - eapply F.relfs_get_r in H1 as [? ?]; eauto 2;
           intuition; eauto 2.
