deps/poulet4/lib/P4cub/Metamorphosis.v
@@ -1,0 +1,413 @@
+Require Import Coq.PArith.BinPos
+        Coq.ZArith.BinInt Coq.NArith.BinNat
+        Poulet4.AList.
+Require Poulet4.P4String Poulet4.P4Int.
+Require Export Poulet4.Typed
+        Poulet4.Syntax Poulet4.P4cub.Syntax.AST.
+Require Import Poulet4.P4cub.Syntax.CubNotations.
+Import AllCubNotations.
+
+Require Import Coq.Strings.String
+        Coq.Classes.EquivDec Poulet4.Monads.Error.
+
+(** * P4light -> P4cub *)
+
+(* General Unresolved Challenges:
+   - What to do about [Locator]?
+     Should p4cub use it?
+   - How should parametric
+     polymorphism be translated?
+   - Should there be fresh string generation,
+     & if so, how to implement it? *)
+
+Section Metamorphosis.
+  Context {tags_t : Type}.
+
+  (* Error type for fine-grained translation errors *)
+  Inductive MorphError :=
+    | Inconceivable (msg: string)
+    | UnsupportedTy (ty: @P4Type tags_t)
+    | UnsupportedExpr (e: @Expression tags_t)
+    | UnsupportedStmt (s: @Statement tags_t)
+    | UnsupportedBop (o: OpBin).
+
+  (** Type Metamorphosis.
+      QUESTIONS:
+      - Why do controls & functions have both
+        constructors in P4Type and their own
+        singleton types?
+      - What to do about parametric polymorphism?
+      - How exactly will types for
+        controls, functions, parsers, actions, tables, & externs be
+        translated? How will they be mapped to
+        p4cub's constructor types?
+      - How, when, & where will [TInteger] be casted?
+      - Should &, if so, how will
+        header unions, strings, enums, varbits, & sets be compiled?
+      - Why is there both a record and a struct type? *)
+  Fixpoint type_morph (t : P4Type) : @error_monad MorphError Expr.t :=
+    let fix lrec (ts : list P4Type) : @error_monad MorphError (list Expr.t) :=
+        match ts with
+        | []     => mret []
+        | t :: ts => t <- type_morph t ;;
+                   ts <- lrec ts ;;
+                   mret (t :: ts)
+        end in
+    let fix frec (fs : P4String.AList tags_t P4Type) : @error_monad MorphError (F.fs string Expr.t) :=
+        match fs with
+        | []         => mret []
+        | (x,t) :: fs => t <- type_morph t ;;
+                       fs <- frec fs ;;
+                       mret ((P4String.str x, t) :: fs)
+        end in
+    match t with
+    | TypBool => mret {{ Bool }}
+    | TypInteger => err (UnsupportedTy t) (* TODO *)
+    | TypString => err (UnsupportedTy t) (* TODO *)
+    | TypInt w => mret $ Expr.TInt $ Pos.of_nat w
+    | TypBit w => mret $ Expr.TBit $ Pos.of_nat w
+    | TypVarBit _ => err (UnsupportedTy t) (* TODO *)
+    | TypArray t n =>
+      let n := Pos.of_nat n in
+      t' <- type_morph t ;;
+      match t' with
+      | {{ hdr { ts } }} => mret {{ stack ts[n] }}
+      | _ => err (UnsupportedTy t)
+      end
+    | TypTuple ts
+    | TypList  ts => ts <<| lrec ts ;; {{ tuple ts }}
+    | TypRecord fs
+    | TypStruct fs => fs <<| frec fs ;; {{ struct { fs } }}
+    | TypSet t' => type_morph t' (* TODO this is a hack that works for well-behaved parsers, but not in general *)
+    | TypError => mret {{ error }}
+    | TypMatchKind => mret {{ matchkind }}
+    | TypVoid => err (UnsupportedTy t) (* TODO *)
+    | TypHeader fs => fs <<| frec fs ;; {{ hdr { fs } }}
+    | TypHeaderUnion _ => err (UnsupportedTy t) (* TODO *)
+    | TypEnum _ _ _ => err (UnsupportedTy t) (* TODO *)
+    | TypTypeName _ => err (UnsupportedTy t) (* TODO *)
+    | TypNewType _ t => type_morph t
+    | TypControl _ => err (UnsupportedTy t) (* TODO *)
+    | TypParser _  => err (UnsupportedTy t) (* TODO *)
+    | TypExtern _  => err (UnsupportedTy t) (* TODO *)
+    | TypFunction _ => err (UnsupportedTy t) (* TODO *)
+    | TypAction _ _ => err (UnsupportedTy t) (* TODO *)
+    | TypTable _ => err (UnsupportedTy t) (* TODO *)
+    | TypPackage _ _ _ => err (UnsupportedTy t) (* TODO *)
+    | TypSpecializedType _ _ => err (UnsupportedTy t) (* TODO, type subsitution? *)
+    | TypConstructor _ _ _ _ => err (UnsupportedTy t) (* TODO, type subsitution? *)
+    end.
+  (**[]*)
+
+  (** Unary Operations *)
+  Definition uop_morph (op : OpUni) : Expr.uop :=
+    match op with
+    | Not => Expr.Not
+    | BitNot => Expr.BitNot
+    | UMinus => Expr.UMinus
+    end.
+  (**[]*)
+
+  (** Binary Operations. *)
+  Definition bop_morph (op : OpBin) : @error_monad MorphError Expr.bop :=
+    match op with
+    | Plus => mret Expr.Plus
+    | PlusSat => mret Expr.PlusSat
+    | Minus => mret Expr.Minus
+    | MinusSat => mret Expr.MinusSat
+    | Mul => mret Expr.Times
+    | Div => err (UnsupportedBop op)
+    | Mod => err (UnsupportedBop op)
+    | Shl => mret Expr.Shl
+    | Shr => mret Expr.Shr
+    | Le => mret Expr.Le
+    | Ge => mret Expr.Ge
+    | Lt => mret Expr.Lt
+    | Gt => mret Expr.Gt
+    | Eq => mret Expr.Eq
+    | NotEq => mret Expr.NotEq
+    | BitAnd => mret Expr.BitAnd
+    | BitXor => mret Expr.BitXor
+    | BitOr => mret Expr.BitOr
+    | PlusPlus => mret Expr.PlusPlus
+    | And => mret Expr.And
+    | Or => mret Expr.Or
+    end.
+  (**[]*)
+
+  (** Expression Metamorphosis.
+      Questions:
+      1. How to translate expressions for:
+         - integers?
+         - strings?
+         - type members [ExpTypemember]?
+         - ternary expressions?
+         - function calls?
+         - nameless instantiations?
+         - don't care expressions?
+         - masks?
+         - ranges?
+      2. Is [P4Name.t] now redundant by [Locator]?
+      3. How to translate [Locator]s?
+      4. Should p4cub's header stack accesses
+         be restricted to compile-time-known indices?
+         From 8.17 "Operations on header stacks",
+         "Some implementations may impose the constraint that the
+          index expression evaluates to a compile-time known value.
+          A P4 compiler must give an error if an index value that is
+          a compile-time constant is out of range".
+          Otherwise progress needs more assumptions.
+      5. Why is [N] still used in [Syntax.v]?
+         Didn't we decide it was undesirable to
+         use both [N] and [Z]? *)
+  Fixpoint expr_morph (e : Expression) : @error_monad MorphError (Expr.e tags_t) :=
+    let fix lstruct (es : list Expression) : @error_monad MorphError (list (Expr.e tags_t)) :=
+        match es with
+        | []     => mret []
+        | e :: es => e <- expr_morph e ;;
+                   es <<| lstruct es ;; e :: es
+        end in
+    let fix frec (fs : list KeyValue)
+        : @error_monad MorphError (F.fs string (Expr.e tags_t)) :=
+        match fs with
+        | [] => mret []
+        | (MkKeyValue _ x e) :: fs
+          => e <- expr_morph e ;;
+            fs <<| frec fs ;;
+            (P4String.str x, e) :: fs
+        end in
+    match e with
+    | MkExpression i (ExpBool b) _ _ => mret <{ BOOL b @ i }>
+    | MkExpression i (ExpInt n)  _ _
+      => let z := P4Int.value n in
+        match P4Int.width_signed n with
+        | Some (w, false) => let w := Pos.of_nat w in mret <{ w W z @ i }>
+        | Some (w, true)  => let w := Pos.of_nat w in mret <{ w S z @ i }>
+        | None => err (UnsupportedExpr e)
+        end
+    | MkExpression i (ExpName (BareName x) _) t _
+      => t <<| type_morph t ;;
+        Expr.EVar t (P4String.str x) i
+    | MkExpression i (ExpArrayAccess e1 e2) t _
+      => t <- type_morph t ;;
+        e1 <- expr_morph e1 ;;
+        e2' <- expr_morph e2 ;;
+        match t, e2' with
+        | {{ hdr { ts } }}, <{ _ W idx @ _ }> => mret <{ Access e1[idx] : ts @ i }>
+        | _, _ => err $ UnsupportedExpr e2 (* TODO *)
+        end
+    | MkExpression i (ExpBitStringAccess e lo hi) _ _
+      => let lo := Pos.pred $ N.succ_pos lo in
+        let hi := Pos.pred $ N.succ_pos hi in
+        e <<| expr_morph e ;; <{ Slice e [hi:lo] @ i }>
+    | MkExpression i (ExpList es) _ _
+      => es <<| lstruct es ;; <{ tup es @ i }>
+    | MkExpression i (ExpRecord fs) _ _
+      => fs <<| frec fs ;; <{ struct { fs } @ i }>
+    | MkExpression i (ExpUnaryOp op e) t _
+      => t <- type_morph t ;;
+        e <<| expr_morph e ;;
+        Expr.EUop t (uop_morph op) e i
+    | MkExpression i (ExpBinaryOp op (e1, e2)) t _
+      => t <-  type_morph t ;;
+        op <- bop_morph op ;;
+        e1 <- expr_morph e1 ;;
+        e2 <<| expr_morph e2 ;; <{ BOP e1 op e2 : t @ i }>
+    | MkExpression i (ExpCast t e) _ _
+      => t <- type_morph t ;;
+        e <<| expr_morph e ;; <{ Cast e:t @ i }>
+    | MkExpression i (ExpErrorMember err) _ _
+      => mret $ Expr.EError (mret $ P4String.str err) i
+    | MkExpression i (ExpExpressionMember e f) t _ 
+      => let f := P4String.str f in
+        t <- type_morph t ;;
+        e <<| expr_morph e ;; 
+        <{ Mem e dot f : t @ i }>
+    | _ => err (UnsupportedExpr e)
+    end.
+  (**[]*)
+
+  Definition type_expr_morph (e : Expression) : @error_monad MorphError (Expr.t * Expr.e tags_t) :=
+    match e with
+    | MkExpression i _ t _ => t <- type_morph t ;;
+                             e <<| expr_morph e ;; (t, e)
+    end.
+  (**[]*)
+
+  Open Scope string_scope.
+  (** Statement Metamorphosis.
+      Questions:
+      1. How should p4cub deal with constants?
+         Should p4cub have constatnts?
+      2. How to translate:
+         - blocks? Should p4cub have blocks?
+         - direct applications?
+           The name of the control being applied
+           is not in [Syntax.v] nor [Typed.v]?
+         - method calls? Type subsitution?
+      3. How to get parameter names to generate arguments?
+      4. When and how will instantiations be lifted? *)
+  Fixpoint stmt_morph (s : Statement) : @error_monad MorphError (Stmt.s tags_t) :=
+    let fix blk_morph (blk : Block) : @error_monad MorphError (Stmt.s tags_t) :=
+        match blk with
+        | BlockEmpty i => mret -{ skip @ i }-
+        | BlockCons ((MkStatement i _ _) as s) blk
+          => s1 <- stmt_morph s ;;
+            s2 <<| blk_morph blk ;; -{ s1; s2 @ i }-
+        end in
+    (* let fix switch_case_morph (swcase : StatementSwitchCase) : option (Stmt.s tags_t) :=
+        match swcase with
+        end in *)
+    match s with
+    | MkStatement i StatEmpty _ => mret -{ skip @ i }-
+    | MkStatement i StatExit  _ => mret -{ exit @ i }-
+    | MkStatement i (StatReturn None) _ => mret -{ return None @ i }-
+    | MkStatement i (StatReturn (Some e)) _ =>
+      e <<| expr_morph e ;; Stmt.SReturn (Some e) i
+    | MkStatement i (StatVariable t x None _) _ =>
+      t <<| type_morph t ;;
+      let x := P4String.str x in
+      -{ delcare x : t @ i }-
+    | MkStatement i (StatVariable _ x (Some e) _) _
+      => e <<| expr_morph e ;;
+        let x := P4String.str x in
+        -{ init x := e @ i }-
+    | MkStatement i (StatAssignment e1 e2) _
+      => e1 <- expr_morph e1 ;;
+        e2 <<| expr_morph e2 ;; -{ asgn e1 := e2 @ i }-
+    | MkStatement i (StatBlock blk) _ => s <<| blk_morph blk ;; -{ b{ s }b }-
+    | MkStatement i (StatConditional e s1 None) _
+      => e <- expr_morph e ;;
+        s1 <<| stmt_morph s1 ;;
+        -{ if e then s1 else skip @ i @ i }-
+    | MkStatement i (StatConditional e s1 (Some s2)) _
+      => e <- expr_morph e ;;
+        s1 <- stmt_morph s1 ;;
+        s2 <<| stmt_morph s2 ;;
+        -{ if e then s1 else s2 @ i }-
+        (*
+    | MkStatement
+        i (StatMethodCall
+             (MkExpression _ 
+                (ExpExpressionMember 
+                  (MkExpression _ 
+                    (ExpName (BareName x) _) 
+                    (TypTypeName (BareName xty)) 
+                    _)
+                  fname)
+                (TypFunction (MkFunctionType _ _ FunExtern retty))
+                _)
+              _
+              args)
+        _
+      =>
+        let x := P4String.str x in 
+        let xty := P4String.str xty in 
+        let fname := P4String.str fname in 
+        if xty == "packet_in" 
+        then
+          args' <- 
+            match args with 
+            | Some e :: nil => 
+              mret (("arg", PAOut (expr_morph e)) :: nil)
+            | _ => mret nil
+            end ;;
+          let ty' := mret None in
+          -{ extern x calls fname <[]> (args') gives ty' @ i }-
+        else err (UnsupportedStmt s) *)
+    | MkStatement i (StatSwitch e cases) _
+      => e <- expr_morph e ;; err (UnsupportedStmt s) (* TODO *)
+    | MkStatement _ _ _ => err (UnsupportedStmt s)
+    end.
+  (**[]*)
+
+  Definition parser_case_morph 
+    (c: @ParserCase tags_t) 
+    : @error_monad MorphError (Parser.pat * string) :=
+    let 'MkParserCase tag matches next := c in 
+    let combine_pats := fun (p: list Parser.pat) =>
+      match p with 
+      | pat :: nil => mret pat
+      | _ :: _ => mret [{ PTUP p }]
+      | nil => err $ Inconceivable "missing pattern base case"
+      end in
+    let match_worker (m: Match) := 
+      let 'MkMatch tag m' ty := m in 
+      match m' with 
+      | MatchDontCare => mret [{ ?? }]
+      | MatchExpression me => 
+        e' <- expr_morph me ;; 
+        match e' with 
+        | <{ w W n @ _ }> => mret [{ w PW n }]
+        | <{ w S n @ _ }> => mret [{ w PS n }]
+        | _ => err $ UnsupportedExpr me
+        end
+      end in 
+    pats <- sequence (map match_worker matches) ;;
+    pats' <- combine_pats pats ;;
+    mret (pats', P4String.str next).
+
+
+  Definition morph_str (n: string) := 
+    match n with 
+    | "start" => ={ start }=
+    | "accept" => ={ accept }=
+    | "reject" => ={ reject }=
+    | name => ={ δ name }=
+    end.
+
+    Definition morph_name (n: P4String.t tags_t) := morph_str (P4String.str n).
+
+  Fixpoint get_default 
+    (tag: tags_t) 
+    (cases: list (Parser.pat * string)) 
+    : @error_monad MorphError (Parser.e tags_t) :=
+    match cases with 
+    | nil => err $ Inconceivable "missing default case in parser select"
+    | ([{ ?? }], s) :: _ => 
+      let st := morph_str s in 
+      mret p{ goto st @ tag }p
+    | _ :: cases => get_default tag cases
+    end.
+
+  Definition morph_cexpr 
+    (tag: tags_t)
+    (x: Parser.pat * string) 
+    : Parser.pat * (Parser.e tags_t) := 
+    let '(pat, nxt) := x in 
+    let st := morph_str nxt in 
+    let nxt_jump := p{ goto st @ tag }p in 
+    (pat, nxt_jump). 
+
+  Definition parser_trans_morph
+    (t: @ParserTransition tags_t)
+    : @error_monad MorphError (Parser.e tags_t) :=
+    match t with 
+    | ParserDirect tag next_name => 
+      let st := morph_name next_name in 
+      mret p{ goto st @ tag }p
+    | ParserSelect tag es cases =>
+      cub_cases <- sequence (map parser_case_morph cases) ;; 
+      cub_exprs <- sequence (map expr_morph es) ;;
+      def <- get_default tag cub_cases ;;
+      let exp := Expr.ETuple cub_exprs tag in 
+      let cub_cases' := map (fun '(k, v) => let v' := morph_str v in (k, p{ goto v' @ tag }p)) cub_cases in 
+      mret p{ select exp { cub_cases' } default := def @ tag }p
+    end.
+
+  Fixpoint combine_ss (tag: tags_t) (ss: list (Stmt.s tags_t)) : Stmt.s tags_t := 
+    match ss with 
+    | nil => -{ skip @ tag }-
+    | s :: ss' => 
+      Stmt.SSeq s (combine_ss tag ss') tag
+    end.
+
+  Definition parser_state_morph 
+    (ps: @ParserState tags_t) 
+    : @error_monad MorphError (string * Parser.state_block tags_t) :=
+    let 'MkParserState tag name ss trans := ps in 
+    ss' <- sequence (map stmt_morph ss) ;; 
+    trans' <- parser_trans_morph trans ;; 
+    mret (P4String.str name, Parser.State (combine_ss tag ss') trans').
+
+End Metamorphosis.
