deps/poulet4/lib/Platform/Packet.v
@@ -2,14 +2,13 @@ Require Import Coq.Bool.Bvector.
 Require Import Coq.Strings.String.
 Require Import Coq.Lists.List.
 Require Import Coq.ZArith.BinIntDef.
-Require Import Coq.NArith.BinNat.
 
 Require Import Poulet4.Monads.Monad.
 Require Import Poulet4.Monads.State.
 
 Require Import Poulet4.Environment.Environment.
 Require Import Poulet4.Utils.
-Require Import Poulet4.Value.
+Require Import Poulet4.Syntax.
 Require Import Poulet4.Typed.
 Require Import Poulet4.Bitwise.
 Require Import Poulet4.AList.
@@ -18,11 +17,9 @@ Open Scope monad.
 Open Scope string_scope.
 
 Section Packet.
-  Context (bit: Type).
-  Context (inject_bit: bool -> bit).
   Context (tags_t: Type).
   Notation P4String := (P4String.t tags_t).
-  Notation ValueBase := (@ValueBase tags_t bit).
+  Notation ValueBase := (@ValueBase tags_t).
   Notation P4Type := (@P4Type tags_t).
 
   Definition packet_monad := @state_monad (list bool) exception.
@@ -54,21 +51,21 @@ Section Packet.
     | TypBool =>
       let* vec := read_first_bits 1 in
       match vec with
-      | (bit :: [])%vector => mret (ValBaseBool (inject_bit bit))
+      | (bit :: [])%vector => mret (ValBaseBool bit)
       | _ => state_fail Internal (* Does not happen -- vec has length exactly 1. *)
       end
     | TypBit width =>
-      let* vec := read_first_bits (N.to_nat width) in
-      mret (ValBaseBit (List.map inject_bit (Vector.to_list vec)))
+      let* vec := read_first_bits width in
+      mret (ValBaseBit width (convert_bits width vec))
     | TypInt width =>
-      let* vec := read_first_bits (N.to_nat width) in
-      mret (ValBaseInt (List.map inject_bit (Vector.to_list vec)))
+      let* vec := read_first_bits width in
+      mret (ValBaseInt width (convert_bits width vec))
     | TypRecord field_types =>
       let* field_vals := sequence (List.map eval_packet_extract_fixed_field field_types) in
       mret (ValBaseRecord field_vals)
     | TypHeader field_types =>
       let* field_vals := sequence (List.map eval_packet_extract_fixed_field field_types) in
-      mret (ValBaseHeader field_vals (inject_bit true))
+      mret (ValBaseHeader field_vals true)
     | _ => state_fail (TypeError "Unsupported type passed to extract.")
     end.
 
@@ -85,5 +82,7 @@ Section Packet.
     | TypInt _ => true
     | _ => false
     end.
+
+
 
 End Packet.
