deps/poulet4/lib/Syntax.v
@@ -57,9 +57,9 @@ Section Syntax.
 
   Definition NoLocator := LGlobal nil.
 
-  (* Inductive KeyValue :=
-  | MkKeyValue (tags: tags_t) (key: P4String) (value: Expression) *)
-  Inductive ExpressionPreT :=
+  Inductive KeyValue :=
+  | MkKeyValue (tags: tags_t) (key: P4String) (value: Expression)
+  with ExpressionPreT :=
   | ExpBool (b: bool)
   | ExpInt (_: P4Int)
   | ExpString (_: P4String)
@@ -67,7 +67,7 @@ Section Syntax.
   | ExpArrayAccess (array: Expression) (index: Expression)
   | ExpBitStringAccess (bits: Expression) (lo: N) (hi: N)
   | ExpList (value: list Expression)
-  | ExpRecord (entries: P4String.AList tags_t Expression)
+  | ExpRecord (entries: list KeyValue)
   | ExpUnaryOp (op: OpUni) (arg: Expression)
   | ExpBinaryOp (op: OpBin) (args: (Expression * Expression))
   | ExpCast (typ: @P4Type tags_t) (expr: Expression)
@@ -79,14 +79,14 @@ Section Syntax.
                     (args: list (option Expression))
   | ExpNamelessInstantiation (typ: @P4Type tags_t) (args: list Expression)
   | ExpDontCare
+  | ExpMask (expr: Expression) (mask: Expression)
+  | ExpRange (lo: Expression) (hi: Expression)
   with Expression :=
   | MkExpression (tags: tags_t) (expr: ExpressionPreT) (typ: @P4Type tags_t) (dir: direction).
 
   Inductive MatchPreT :=
   | MatchDontCare
-  | MatchMask (expr: Expression) (mask: Expression)
-  | MatchRange (lo: Expression) (hi: Expression)
-  | MatchCast (typ: @P4Type tags_t) (expr: Expression).
+  | MatchExpression (expr: Expression).
 
   Inductive Match :=
   | MkMatch (tags: tags_t) (expr: MatchPreT) (typ: @P4Type tags_t).
@@ -110,6 +110,36 @@ Section Syntax.
   Inductive TableProperty :=
   | MkTableProperty (tags: tags_t)  (const: bool)
                     (name: P4String) (value: Expression).
+
+  Inductive ValueBase :=
+  | ValBaseNull
+  | ValBaseBool (_: bool)
+  | ValBaseInteger (_: Z)
+  | ValBaseBit (width: nat) (value: Z)
+  | ValBaseInt (width: nat) (value: Z)
+  | ValBaseVarbit (max: nat) (width: nat) (value: Z)
+  | ValBaseString (_: P4String)
+  | ValBaseTuple (_: list ValueBase)
+  | ValBaseRecord (_: P4String.AList tags_t ValueBase)
+  | ValBaseSet (_: ValueSet)
+  | ValBaseError (_: P4String)
+  | ValBaseMatchKind (_: P4String)
+  | ValBaseStruct (fields: P4String.AList tags_t ValueBase)
+  | ValBaseHeader (fields: P4String.AList tags_t ValueBase) (is_valid: bool)
+  | ValBaseUnion (fields: P4String.AList tags_t ValueBase)
+  | ValBaseStack (headers: list ValueBase) (size: nat) (next: nat)
+  | ValBaseEnumField (typ_name: P4String) (enum_name: P4String)
+  | ValBaseSenumField (typ_name: P4String) (enum_name: P4String) (value: ValueBase)
+  | ValBaseSenum (_: P4String.AList tags_t ValueBase)
+  with ValueSet :=
+  | ValSetSingleton (value: ValueBase)
+  | ValSetUniversal
+  | ValSetMask (value: ValueBase) (mask: ValueBase)
+  | ValSetRange (lo: ValueBase) (hi: ValueBase)
+  | ValSetProd (_: list ValueSet)
+  | ValSetLpm (width: ValueBase) (nbits: nat) (value: ValueBase)
+  | ValSetValueSet (size: ValueBase) (members: list (list Match))
+                   (sets: list ValueSet).
 
   Inductive StatementSwitchLabel :=
   | StatSwLabDefault (tags: tags_t)
@@ -139,7 +169,7 @@ Section Syntax.
   | StatSwitch (expr: Expression)
                (cases: list StatementSwitchCase)
   | StatConstant  (typ: @P4Type tags_t)
-                  (name: P4String) (value: Expression)
+                  (name: P4String) (value: ValueBase)
                   (loc: Locator)
   | StatVariable  (typ: @P4Type tags_t)
                   (name: P4String) (init: option Expression)
@@ -346,7 +376,7 @@ Section Syntax.
 
   Inductive Declaration :=
   | DeclConstant (tags: tags_t)  (typ: @P4Type tags_t)
-                 (name: P4String) (value: Expression)
+                 (name: P4String) (value: ValueBase)
   | DeclInstantiation (tags: tags_t)  (typ: @P4Type tags_t)
                       (args: list Expression) (name: P4String) (init: list Declaration)
   | DeclParser (tags: tags_t)  (name: P4String)
@@ -365,14 +395,14 @@ Section Syntax.
   | DeclVariable (tags: tags_t)  (typ: @P4Type tags_t)
                  (name: P4String) (init: option Expression)
   | DeclValueSet (tags: tags_t)  (typ: @P4Type tags_t)
-                 (size: N) (name: P4String)
+                 (size: Expression) (name: P4String)
   | DeclAction (tags: tags_t)  (name: P4String)
                (data_params: list (@P4Parameter tags_t)) (ctrl_params: list (@P4Parameter tags_t))
                (body: Block)
   | DeclTable (tags: tags_t)  (name: P4String)
               (key: list TableKey) (actions: list TableActionRef)
               (entries: option (list TableEntry))
-              (default_action: option TableActionRef) (size: option N)
+              (default_action: option TableActionRef) (size: option P4Int)
               (custom_properties: list TableProperty)
   | DeclHeader (tags: tags_t)  (name: P4String)
                (fields: list DeclarationField)
@@ -399,6 +429,138 @@ Section Syntax.
   | DeclPackageType (tags: tags_t)  (name: P4String)
                     (type_params: list P4String) (params: list (@P4Parameter tags_t)).
 
+  Section declaration_rec.
+    Context
+      {PDeclaration : Declaration -> Type}
+      {PDeclarationList : list Declaration -> Type}
+    .
+
+    Hypotheses
+      (HDeclConstant: forall tags typ name value,
+          PDeclaration (DeclConstant tags typ name value))
+      (HDeclInstantiation: forall tags typ args name init,
+          PDeclarationList init ->
+          PDeclaration (DeclInstantiation tags typ args name init))
+      (HDeclParser: forall tags name type_params params constructor_params locals states,
+          PDeclaration (DeclParser tags name type_params params constructor_params locals states))
+      (HDeclControl: forall tags name type_params params constructor_params locals apply,
+          PDeclaration (DeclControl tags name type_params params constructor_params locals apply))
+      (HDeclFunction: forall tags ret name type_params params body,
+          PDeclaration (DeclFunction tags ret name type_params params body))
+      (HDeclExternFunction: forall tags ret name type_params params,
+          PDeclaration (DeclExternFunction tags ret name type_params params))
+      (HDeclVariable: forall tags typ name init,
+          PDeclaration (DeclVariable tags typ name init))
+      (HDeclValueSet: forall tags typ size name,
+          PDeclaration (DeclValueSet tags typ size name))
+      (HDeclAction: forall tags name data_params ctrl_params body,
+          PDeclaration (DeclAction tags name data_params ctrl_params body))
+      (HDeclTable: forall tags name key actions entries default_action size custom_properties,
+          PDeclaration (DeclTable tags name key actions entries default_action size custom_properties))
+      (HDeclHeader: forall tags name fields,
+          PDeclaration (DeclHeader tags name fields))
+      (HDeclHeaderUnion: forall tags name fields,
+          PDeclaration (DeclHeaderUnion tags name fields))
+      (HDeclStruct: forall tags name fields,
+          PDeclaration (DeclStruct tags name fields))
+      (HDeclError: forall tags members,
+          PDeclaration (DeclError tags members))
+      (HDeclMatchKind: forall tags members,
+          PDeclaration (DeclMatchKind tags members))
+      (HDeclEnum: forall tags name members,
+          PDeclaration (DeclEnum tags name members))
+      (HDeclSerializableEnum: forall tags typ name members,
+          PDeclaration (DeclSerializableEnum tags typ name members))
+      (HDeclExternObject: forall tags name type_params methods,
+          PDeclaration (DeclExternObject tags name type_params methods))
+      (HDeclTypeDef: forall tags name typ_or_decl,
+          PDeclaration (DeclTypeDef tags name typ_or_decl))
+      (HDeclNewType: forall tags name typ_or_decl,
+          PDeclaration (DeclNewType tags name typ_or_decl))
+      (HDeclControlType: forall tags name type_params params,
+          PDeclaration (DeclControlType tags name type_params params))
+      (HDeclParserType: forall tags name type_params params,
+          PDeclaration (DeclParserType tags name type_params params))
+      (HDeclPackageType: forall tags name type_params params,
+          PDeclaration (DeclPackageType tags name type_params params))
+      (HDeclarationListNil: PDeclarationList nil)
+      (HDeclarationListCons: forall hd tl,
+          PDeclaration hd ->
+          PDeclarationList tl ->
+          PDeclarationList (cons hd tl)).
+
+    Fixpoint declaration_rec (decl : Declaration) :=
+      match decl with
+      | DeclConstant tags typ name value =>
+        HDeclConstant tags typ name value
+      | DeclInstantiation tags typ args name init =>
+        HDeclInstantiation tags typ args name init
+        (list_rec
+          PDeclaration
+          PDeclarationList
+          HDeclarationListNil
+          HDeclarationListCons
+          declaration_rec
+          init
+        )
+      | DeclParser tags name type_params params constructor_params locals states =>
+        HDeclParser tags name type_params params constructor_params locals states
+      | DeclControl tags name type_params params constructor_params locals apply =>
+        HDeclControl tags name type_params params constructor_params locals apply
+      | DeclFunction tags ret name type_params params body =>
+        HDeclFunction tags ret name type_params params body
+      | DeclExternFunction tags ret name type_params params =>
+        HDeclExternFunction tags ret name type_params params
+      | DeclVariable tags typ name init =>
+        HDeclVariable tags typ name init
+      | DeclValueSet tags typ size name =>
+        HDeclValueSet tags typ size name
+      | DeclAction tags name data_params ctrl_params body =>
+        HDeclAction tags name data_params ctrl_params body
+      | DeclTable tags name key actions entries default_action size custom_properties =>
+        HDeclTable tags name key actions entries default_action size custom_properties
+      | DeclHeader tags name fields =>
+        HDeclHeader tags name fields
+      | DeclHeaderUnion tags name fields =>
+        HDeclHeaderUnion tags name fields
+      | DeclStruct tags name fields =>
+        HDeclStruct tags name fields
+      | DeclError tags members =>
+        HDeclError tags members
+      | DeclMatchKind tags members =>
+        HDeclMatchKind tags members
+      | DeclEnum tags name members =>
+        HDeclEnum tags name members
+      | DeclSerializableEnum tags typ name members =>
+        HDeclSerializableEnum tags typ name members
+      | DeclExternObject tags name type_params methods =>
+        HDeclExternObject tags name type_params methods
+      | DeclTypeDef tags name typ_or_decl =>
+        HDeclTypeDef tags name typ_or_decl
+      | DeclNewType tags name typ_or_decl =>
+        HDeclNewType tags name typ_or_decl
+      | DeclControlType tags name type_params params =>
+        HDeclControlType tags name type_params params
+      | DeclParserType tags name type_params params =>
+        HDeclParserType tags name type_params params
+      | DeclPackageType tags name type_params params =>
+        HDeclPackageType tags name type_params params
+      end.
+
+  End declaration_rec.
+
+  Definition ValueLoc := P4String.
+
+  Inductive ValueTable :=
+  | MkValTable (name: P4String) (keys: list TableKey)
+               (actions: list TableActionRef) (default_action: TableActionRef)
+               (const_entries: list TableEntry).
+
+  Definition Env_env binding := list (P4String.AList tags_t binding).
+
+  Inductive Env_EvalEnv :=
+  | MkEnv_EvalEnv (vs: Env_env ValueLoc) (typ: Env_env (@P4Type tags_t)) (namespace: P4String).
+
   Record ExternMethod :=
     { name: P4String;
       typ: @FunctionType tags_t }.
@@ -407,6 +569,51 @@ Section Syntax.
     { type_params: list P4String;
       methods: list ExternMethod;
       abst_methods: list ExternMethod }.
+
+  Inductive ValuePreLvalue :=
+  | ValLeftName (name: @Typed.name tags_t) (loc: Locator)
+  | ValLeftMember (expr: ValueLvalue) (name: P4String)
+  | ValLeftBitAccess (expr: ValueLvalue) (msb: nat) (lsb: nat)
+  | ValLeftArrayAccess (expr: ValueLvalue) (idx: nat)
+  with ValueLvalue :=
+  | MkValueLvalue (lvalue: ValuePreLvalue) (typ: @P4Type tags_t).
+
+  Inductive ValueFunctionImplementation :=
+  | ValFuncImplUser (scope: Env_EvalEnv) (body: Block)
+  | ValFuncImplExtern (name: P4String) (caller: option (ValueLoc * P4String))
+  | ValFuncImplBuiltin (name: P4String) (caller: ValueLvalue).
+
+  Inductive ValueObject :=
+  | ValObjParser (scope: Env_EvalEnv)
+                 (constructor_params: list (@P4Parameter tags_t))
+                 (params: list (@P4Parameter tags_t)) (locals: list Declaration)
+                 (states: list ParserState)
+  | ValObjTable (_: ValueTable)
+  | ValObjControl (scope: Env_EvalEnv)
+                  (constructor_params: list (@P4Parameter tags_t))
+                  (params: list (@P4Parameter tags_t)) (locals: list Declaration)
+                  (apply: Block)
+  | ValObjPackage (args: P4String.AList tags_t ValueLoc)
+  | ValObjRuntime (loc: ValueLoc) (obj_name: P4String)
+  | ValObjFun (params: list (@P4Parameter tags_t)) (impl: ValueFunctionImplementation)
+  | ValObjAction (scope: Env_EvalEnv) (params: list (@P4Parameter tags_t)) (body: Block)
+  | ValObjPacket (bits: list bool).
+
+  Inductive ValueConstructor :=
+  | ValConsParser (scope: Env_EvalEnv) (constructor_params: list (@P4Parameter tags_t))
+                  (params: list (@P4Parameter tags_t)) (locals: list Declaration)
+                  (states: list ParserState)
+  | ValConsTable (_: ValueTable)
+  | ValConsControl (scope: Env_EvalEnv) (constructor_params: list (@P4Parameter tags_t))
+                   (params: list (@P4Parameter tags_t)) (locals: list Declaration)
+                   (apply: Block)
+  | ValConsPackage (params: list (@P4Parameter tags_t)) (args: P4String.AList tags_t ValueLoc)
+  | ValConsExternObj (_: P4String.AList tags_t (list (@P4Parameter tags_t))).
+
+  Inductive Value :=
+  | ValBase (_: ValueBase)
+  | ValObj (_: ValueObject)
+  | ValCons (_: ValueConstructor).
 
   Inductive program := Program (_: list Declaration).
 
