deps/poulet4/lib/Target.v
@@ -6,7 +6,6 @@ Require Import Coq.Lists.List.
 Require Import Coq.Program.Program.
 Require Import Poulet4.Typed.
 Require Import Poulet4.Syntax.
-Require Import Poulet4.Value.
 Require Import Poulet4.SyntaxUtil.
 Require Import Poulet4.P4Int.
 Require Import Poulet4.Maps.
@@ -16,27 +15,25 @@ Section Target.
 Context {tags_t: Type}.
 Notation ident := (P4String.t tags_t).
 Notation path := (list ident).
-Notation Val := (@ValueBase tags_t bool).
-Notation ValSet := (@ValueSet tags_t).
+Notation Val := (@ValueBase tags_t).
 Notation signal := (@signal tags_t).
 
-Fixpoint width_of_val (v: Val): N :=
-  let fix fields_width (fields: P4String.AList tags_t ValueBase) : N :=
+Fixpoint width_of_val (v: Val): nat :=
+  let fix fields_width (fields: P4String.AList tags_t ValueBase) : nat :=
       match fields with
-      | nil => N.of_nat O
-      | (id, v) :: rest => (width_of_val v + fields_width rest)%N
+      | nil => O
+      | (id, v) :: rest => width_of_val v + fields_width rest
       end in
   match v with
-  | ValBaseNull => N.of_nat O
+  | ValBaseNull => O
   | ValBaseBool _ => 1
-  | ValBaseBit bits
-  | ValBaseInt bits
-  | ValBaseVarbit _ bits => Z.to_N (Zlength bits)
-  | ValBaseTuple vs => List.fold_right N.add (0)%N (List.map width_of_val vs)
+  | ValBaseBit w _
+  | ValBaseInt w _
+  | ValBaseVarbit _ w _ => w
   | ValBaseStruct fields
   | ValBaseHeader fields _ => fields_width fields
   | ValBaseSenumField _ _ v => width_of_val v
-  | _ => N.of_nat O
+  | _ => O
   end.
 
 (* We want to share the notation of External between P4light and P4cub, so later we need to
@@ -53,34 +50,31 @@ Inductive table_entry :=
   (* TODO replace Expression in Match with Val. *)
   mk_table_entry (matches : list (@Match tags_t)) (action : action_ref).
 
-Definition table_entry_valset : Type :=  ValSet * action_ref.
-
 Class ExternSem := {
-  extern_object : Type;
-  extern_state := @PathMap.t tags_t extern_object;
-  extern_empty := @PathMap.empty tags_t extern_object;
+  extern_state : Type;
+  extern_empty : extern_state;
   (* Allocation should be a function; calling may be fine as a relation. *)
   alloc_extern : extern_state -> ident (* class *) -> list (@P4Type tags_t) -> path -> list Val -> extern_state;
   exec_extern : extern_state -> ident (* class *) -> ident (* method *) -> path -> list (@P4Type tags_t) -> list Val -> extern_state -> list Val -> signal -> Prop;
   extern_get_entries : extern_state -> path -> list table_entry;
-  extern_match : list (Val * ident (* match_kind *)) -> list table_entry_valset -> option action_ref (* action *)
+  extern_match : list (Val * ident (* match_kind *)) -> list table_entry -> option action_ref (* action *)
 }.
 
 Class SeparableExternSem := {
-  ses_extern_object : Type;
+  extern_object : Type;
   (* extern_state := @IdentMap.t tags_t extern_object; *)
   (* extern_empty : extern_state := IdentMap.empty; *)
   (* Allocation should be a function; calling may be fine as a relation. *)
-  ses_alloc_extern : ident (* class *) -> list (@P4Type tags_t) -> list Val -> ses_extern_object;
-  ses_exec_extern : ident (* class *) -> ident (* method *) -> ses_extern_object -> list (@P4Type tags_t) -> list Val -> ses_extern_object -> list Val -> signal -> Prop;
+  ses_alloc_extern : ident (* class *) -> list (@P4Type tags_t) -> list Val -> extern_object;
+  ses_exec_extern : ident (* class *) -> ident (* method *) -> extern_object -> list (@P4Type tags_t) -> list Val -> extern_object -> list Val -> signal -> Prop;
   (* ses_extern_get_entries : extern_state -> path -> list table_entry; *)
-  ses_extern_match : list (Val * ident (* match_kind *)) -> list table_entry_valset -> option action_ref (* action *)
+  ses_extern_match : list (Val * ident (* match_kind *)) -> list table_entry -> option action_ref (* action *)
 }.
 
 Section ExternSemOfSeparableExternSem.
 Context (ses : SeparableExternSem).
 
-(* Definition extern_state' : Type := @PathMap.t tags_t ses_extern_object * @PathMap.t tags_t (list table_entry).
+Definition extern_state' : Type := @PathMap.t tags_t extern_object * @PathMap.t tags_t (list table_entry).
 
 Inductive exec_extern' : extern_state' -> ident (* class *) -> ident (* method *) -> path -> list (@P4Type tags_t) -> list Val -> extern_state' -> list Val -> signal -> Prop :=
   | exec_extern_intro : forall s class method targs p args s' args' vret obj obj',
@@ -96,17 +90,17 @@ Definition extern_get_entries' (s : extern_state') p :=
   end.
 
 Definition ExternSemOfSeparableExternSem := {|
-  extern_object := ses_extern_object;
+  extern_state := extern_state';
   extern_empty := (PathMap.empty, PathMap.empty);
   alloc_extern := (fun s class type_params p args =>
                     (PathMap.set p (ses_alloc_extern class type_params args) (fst s), snd s));
   exec_extern := exec_extern';
   extern_get_entries := extern_get_entries';
   extern_match := ses_extern_match
-|}. *)
+|}.
 End ExternSemOfSeparableExternSem.
 
-(* Coercion ExternSemOfSeparableExternSem : SeparableExternSem >-> ExternSem. *)
+Coercion ExternSemOfSeparableExternSem : SeparableExternSem >-> ExternSem.
 
 Class Target := {
   extern_sem :> ExternSem;
